Progress on MS queue

src/examples/durable_ms_queue.v
@@ -3,6 +3,7 @@ Michael-Scott queue. *)
 
 From iris.bi Require Import lib.fractional.
 From iris.proofmode Require Import tactics.
+From iris.bi.lib Require Export fixpoint.
 
 From self.base Require Import primitive_laws.
 From self.lang Require Import lang.
@@ -17,58 +18,11 @@ From self.high Require Import dprop abstract_state_instances modalities
      recovery_weakestpre lifted_modalities protocol protocols no_buffer mapsto_na_flushed.
 From self.high.modalities Require Import fence.
 
-
 (* Implementation. *)
 
 Section implementation.
 
   Notation NONE := (InjL #()).
-
-  (*
-  (* Construct a new empty queue. *)
-  Definition mk_queue : expr :=
-    λ: <>,
-      let: "node" := ref_NA (InjL #()) in
-      Flush "node" ;;
-      Fence ;;
-      let: "toHead" := ref_AT "node" ;;
-      let: "toTail" := ref_AT "node" ;;
-      ("toHead", "toTail").
-
-  Definition enqueue : expr :=
-    λ: "toHead" "val",
-      let: "toNext" := ref_NA #() in
-      let: "newNode" := ref_NA (InjR ("val", "toNext")) in
-      Flush "newNode" ;;
-      (rec: "loop" <> :=
-        let: "head" := !_AT "toHead" in
-        "toNext" <-_NA "head" ;;
-        Flush "toNext" ;;
-        Fence ;;
-        if: CAS "toHead" "head" "newNode"
-        then #()
-        else "loop" #()
-      ) #().
-
-  Definition dequeue : expr :=
-    rec: "loop" "q" :=
-      let: "toHead" := Fst "q" in
-      let: "head" := !_AT "toHead" in
-      Fence ;;
-      match: !_NA "head" with
-        NONE => NONE
-      | SOME "pair" =>
-          let: "nextNode" := !_NA (Snd "pair") in
-          if: CAS "toHead" "head" "nextNode"
-          then SOME (Fst "pair")
-          else "loop" "toHead"
-      end.
-  *)
-
-  (* Definition sync : expr := *)
-  (*   λ: "toHead", *)
-  (*     Flush "toHead" ;; *)
-  (*     FenceSync. *)
 
   Definition MS_nilv := NONEV.
   Definition MS_consv x nOut : val := SOMEV ((SOMEV x), nOut).
@@ -99,10 +53,13 @@ Section implementation.
     rec: "try" "queue" :=
       let: "toSent" := Fst "queue" in
       let: "sent" := !_AT "toSent" in
+      Fence ;; (* NOTE: Investigate whether this fence is strictly neccessary. *)
       let: "c" := getValue (!_AT "sent") in
+      Fence ;; (* NOTE: Investigate whether this fence is strictly neccessary. *)
       match: !_AT (!_AT (Snd "c")) with
         NONE => NONE
       | SOME "n'" =>
+          Fence ;;
           if: (CAS "toSent" "sent" (!_AT (Snd "c")))
           then SOME (getValue (Fst ("n'")))
           else "try" #()
@@ -147,20 +104,74 @@ Section definitions.
 
   Definition loc_predO `{nvmG Σ} ST := ST -d> val -d> dPropO Σ.
 
-  Definition toNext_prod_inv (pred : loc_pred bool) :
-      loc_pred (discreteState loc + discreteState loc) :=
+  (* Left injection means pointer to a nil node, and right means pointer to a
+  cons node. Due to the use of [discreteState] the location can only be updated
+  a single time. *)
+  Definition toNext_state : Type := discreteState loc + discreteState loc.
+
+  (* The invariant for the location out of a node. *)
+  Definition toNext_prot_inv (next_inv : loc_predO bool) :
+      loc_predO toNext_state :=
     λ ml v,
       match ml with
         inl (mk_discrete ℓ) =>
-          ⌜ v = #(ℓ : loc) ⌝ ∗ know_pred_d ℓ pred
+          ⌜ v = #(ℓ : loc) ⌝ ∗
+          ℓ ↦_AT^{nil_node_prot} [()] ∗
+          flush_lb ℓ (nil_node_prot) ()
       | inr (mk_discrete ℓ) =>
-          ⌜ v = #ℓ ⌝ ∗ know_pred_d ℓ pred
+          ⌜ v = #ℓ ⌝ ∗
+          ℓ ↦_AT^{MkProt next_inv id} [true] ∗
+          flush_lb ℓ (MkProt next_inv id) true
       end%I.
 
+  Global Instance toNext_prot_inv_ne :
+    NonExpansive toNext_prot_inv.
+  Proof.
+    rewrite /toNext_prot_inv.
+    intros ???? [|[ℓ]] ?; first solve_proper.
+    f_equiv.
+    f_equiv.
+    - rewrite /mapsto_at.
+      f_equiv. f_equiv. f_equiv. f_equiv. f_equiv. f_equiv. f_equiv. f_equiv.
+      f_equiv. f_equiv. f_equiv. f_equiv. f_equiv. f_equiv. f_equiv. f_equiv.
+      f_equiv. f_equiv. f_equiv. f_equiv. f_equiv. f_equiv.
+      rewrite /know_protocol.
+      f_equiv; last done.
+      simpl.
+      f_equiv.
+      rewrite /know_pred_d.
+      f_equiv.
+      intros ?? ->.
+      f_equiv.
+      assumption.
+    - rewrite /flush_lb.
+      f_equiv. f_equiv. f_equiv. f_equiv. f_equiv. f_equiv.
+      rewrite /lb_base.
+      f_equiv.
+      rewrite /know_protocol.
+      f_equiv.
+      f_equiv; last done.
+      f_equiv.
+      rewrite /know_pred_d.
+      f_equiv.
+      intros ?? ->.
+      f_equiv.
+      simpl.
+      assumption.
+  Qed.
+
+  Definition toNext_prot (next_inv : loc_pred bool) :=
+    MkProt (toNext_prot_inv next_inv) id.
+
+  (*
+  Definition TT := (bool * val) -d> dPropO Σ.
+
+  (* bi fixpoint *)
+  (* The invariant for the location into a node. Without later. *)
   Definition pre_node_prot_inv (ℓtoNext : loc) :
-     (loc_predO bool) -d> loc_predO bool :=
-    λ self b v,
-      (∃ mx,
+     (TT) -d> TT :=
+    λ self '(b, v),
+      (∃ mx state,
         ⌜ v = (InjRV (mx, #ℓtoNext)) ⌝ ∗
         match b with
           (* Is initial sentinel. *)
@@ -168,26 +179,196 @@ Section definitions.
           (* Is not a sentinel node. *)
         | true => ∃ x, ⌜ mx = SOMEV x ⌝ ∗ R x
         end ∗
-        ▷ know_pred_d ℓtoNext (toNext_prod_inv self))%I
-    .
+        ℓtoNext ↦_AT^{toNext_prot (λ s v, self (s, v))} [state] ∗
+        flush_lb ℓtoNext (toNext_prot (λ s v, self (s, v))) state)%I.
+
+  (* Global Instance flush_lb_ne : *)
+
+  Instance pre_node_prot_inv_ne ℓ : NonExpansive2 (pre_node_prot_inv ℓ).
+  Proof.
+    intros.
+    intros ??? (?, ?) [??] [<-%leibniz_equiv <-%leibniz_equiv]%pair_equiv_inj.
+    rewrite /pre_node_prot_inv.
+    f_equiv.
+    f_equiv.
+    f_equiv.
+    f_equiv.
+    f_equiv.
+    f_equiv.
+    f_equiv.
+    - admit.
+    - rewrite /flush_lb.
+      f_equiv.
+      f_equiv.
+      f_equiv.
+      f_equiv.
+      f_equiv.
+      f_equiv.
+      rewrite /lb_base.
+      f_equiv.
+      f_equiv.
+      rewrite /know_protocol /know_pred_d /know_bumper.
+      f_equiv.
+      { admit. }
+      f_equiv.
+      f_equiv.
+      f_equiv.
+      admit.
+  Admitted.
+
+  Definition uncurried_node_prot_inv ℓ : TT :=
+    bi_least_fixpoint (pre_node_prot_inv ℓ).
+
+  (* Global Instance name ℓ : BiMonoPred (pre_node_prot_inv ℓ). *)
+  (* Proof. *)
+  (*   split. *)
+  (*   - iIntros (Φ Ψ ??) "#HI". iIntros ([s b]). *)
+  (*     simpl. *)
+  (*     iDestruct 1 as (mx state) "(A & B & C & D)". *)
+  (*     iExists mx, state. *)
+  (*     iFrameF "A". *)
+  (*     iFrameF "B". *)
+  (*     iSplitL "C". *)
+  (*     * rewrite /mapsto_at. *)
+  (*     (* iFrame "%#∗". *) *)
+  (*     admit. *)
+  (*   - *)
+  (* Admitted. *)
+
+  Lemma node_prot_inv_unfold ℓtoNext :
+    uncurried_node_prot_inv ℓtoNext ≡
+      pre_node_prot_inv ℓtoNext (uncurried_node_prot_inv ℓtoNext).
+  Proof.
+    rewrite /uncurried_node_prot_inv.
+    intros ?.
+    apply least_fixpoint_unfold.
+    apply _.
+  Qed.
+*)
+
+  (* WITH LATER The invariant for the location into a node. *)
+  Definition pre_node_prot_inv (ℓtoNext : loc) :
+     (loc_predO bool) -d> loc_predO bool :=
+    λ self b v,
+      (∃ mx state,
+        ⌜ v = (InjRV (mx, #ℓtoNext)) ⌝ ∗
+        match b with
+          (* Is initial sentinel. *)
+          false => True
+          (* Is not a sentinel node. *)
+        | true => ∃ x, ⌜ mx = SOMEV x ⌝ ∗ R x
+        end ∗
+        ℓtoNext ↦_AT^{toNext_prot self} [state] ∗
+        flush_lb ℓtoNext (toNext_prot self) state)%I.
 
   Global Instance pre_node_prot_inv_contractive ℓtoNext :
     Contractive (pre_node_prot_inv ℓtoNext).
   Proof.
-    intros ???? [|].
-    (* solve_contractive. *)
-  Admitted.
+    intros ??????.
+    rewrite /pre_node_prot_inv.
+    (* intros ?. *)
+    simpl.
+    f_equiv.
+    f_equiv.
+    f_equiv.
+    f_equiv.
+    f_equiv.
+    f_equiv.
+    f_equiv.
+    - rewrite /mapsto_at.
+      f_equiv. f_equiv. f_equiv. f_equiv. f_equiv. f_equiv. f_equiv. f_equiv.
+      f_equiv. f_equiv. f_equiv. f_equiv. f_equiv. f_equiv. f_equiv. f_equiv.
+      f_equiv. f_equiv. f_equiv. f_equiv. f_equiv. f_equiv.
+      rewrite /know_protocol.
+      f_equiv; last done.
+      simpl.
+      f_equiv.
+      rewrite /know_pred_d.
+      f_equiv.
+      intros ?? ->.
+      f_contractive.
+      f_equiv.
+      assumption.
+    - rewrite /flush_lb.
+      f_equiv. f_equiv. f_equiv. f_equiv. f_equiv. f_equiv.
+      rewrite /lb_base.
+      f_equiv.
+      rewrite /know_protocol.
+      f_equiv.
+      f_equiv; last done.
+      f_equiv.
+      rewrite /know_pred_d.
+      f_equiv.
+      intros ?? ->.
+      f_contractive.
+      simpl.
+      f_equiv.
+      assumption.
+  Qed.
 
-  Definition node_prot_inv ℓtoNext :=
-    fixpoint (pre_node_prot_inv ℓtoNext).
+  Definition node_prot_inv ℓtoNext := fixpoint (pre_node_prot_inv ℓtoNext).
 
-  Program Definition node_prot (ℓtoNext : loc) : LocationProtocol bool :=
-    {| pred := (node_prot_inv ℓtoNext);
-       bumper := id |}.
-  Next Obligation.
+  Lemma node_prot_inv_unfold ℓtoNext :
+    node_prot_inv ℓtoNext ≡ pre_node_prot_inv ℓtoNext (node_prot_inv ℓtoNext).
+  Proof. rewrite /node_prot_inv. apply fixpoint_unfold. Qed.
 
-  Program Definition cons_node_prot (ℓtoNext : loc) : LocationProtocol bool :=
-    {| pred b v := (∃ mx,
+  Instance if_else_persistent {PROP : bi} (b : bool) (P Q : PROP) :
+    Persistent P →
+    Persistent Q →
+    Persistent (if b then P else Q).
+  Proof. intros ??. destruct b; done. Qed.
+
+  Lemma node_prot_inv_persistent `{∀ v, Persistent (R v)} ℓtoNext s v : Persistent (node_prot_inv ℓtoNext s v).
+  Proof.
+    rewrite /Persistent.
+    (* iLöb as "IH" forall (ℓtoNext s v). *)
+    rewrite /node_prot_inv.
+    rewrite (fixpoint_unfold (pre_node_prot_inv ℓtoNext) s v).
+    iDestruct 1 as (??) "(-> & #HR & #prot & #lb)".
+    iModIntro.
+    iExists _, _.
+    iSplitPure; first done.
+    iFrame "#".
+  Qed.
+
+  Global Instance toNext_prot_inv_persistent ℓtoNext s v :
+    Persistent (toNext_prot_inv (node_prot_inv ℓtoNext) s v).
+  Proof. destruct s as [[?]|[?]]; apply _. Qed.
+
+  Definition cons_node_prot (ℓtoNext : loc) : LocationProtocol bool :=
+    {| p_inv := (node_prot_inv ℓtoNext);
+       p_bumper := id |}.
+
+  Global Instance cons_node_prot_conditions (ℓtoNext : loc) :
+    ProtocolConditions (cons_node_prot ℓtoNext).
+  Proof.
+    split; try apply _.
+    - intros ??. simpl.
+      rewrite /node_prot_inv (fixpoint_unfold (pre_node_prot_inv _) s v).
+      apply _.
+    - iLöb as "IH".
+      iIntros (??) "nodeProt".
+      simpl.
+      rewrite /node_prot_inv.
+      rewrite (fixpoint_unfold (pre_node_prot_inv ℓtoNext) s v).
+      iDestruct "nodeProt" as (??) "(-> & HR & prot & lb)".
+      iModIntro.
+      simpl.
+      iDestruct "lb" as "(persLb & (%state' & #incl & #crashedIn))".
+      iExists mx, state'.
+      iSplitPure; first done.
+      iFrameF "HR".
+      iDestruct (crashed_in_if_rec with "crashedIn prot")
+        as (?) "(crashedIn2 & toNextPts)".
+      iDestruct (crashed_in_agree with "crashedIn crashedIn2") as %<-.
+      iFrame "toNextPts".
+      iApply persist_lb_to_flush_lb.
+      iApply (crashed_in_persist_lb with "crashedIn").
+  Qed.
+
+  (*
+  Definition cons_node_prot (ℓtoNext : loc) : LocationProtocol bool :=
+    {| p_inv b v := (∃ mx,
         ⌜ v = (InjRV (mx, #ℓtoNext)) ⌝ ∗
         (* no info about [ℓtoNext] *)
         (* ℓtoNext ↦_AT^{toNext_prot} [false] ∗ *)
@@ -197,28 +378,33 @@ Section definitions.
           (* Is not a sentinel node. *)
         | true => ∃ x, ⌜ mx = SOMEV x ⌝ ∗ R x
        end)%I;
-       bumper := id
+       p_bumper := id
     |}.
-  Next Obligation. Admitted.
-  Next Obligation. Admitted.
+
+  Global Instance cons_node_prot_conditions ℓtoNext :
+    ProtocolConditions (cons_node_prot ℓtoNext).
+  Proof.
+    split; try apply _.
+  Admitted.
+  *)
 
     (* constant_prot (InjRV (x, #ℓtoNext)). *)
 
-  Program Definition toNext_prot :
-    LocationProtocol ((discreteState loc) + (discreteState loc)) :=
-    {| pred ml v :=
-        ⌜ match ml with
-          inl (mk_discrete ℓ) => v = #ℓ
-        | inr (mk_discrete ℓ) => v = #ℓ
-        end ⌝%I;
-      bumper := id |}.
-  Next Obligation. Admitted.
+  (* Definition toNext_prot : *)
+  (*   LocationProtocol ((discreteState loc) + (discreteState loc)) := *)
+  (*   {| p_inv ml v := *)
+  (*       ⌜ match ml with *)
+  (*         inl (mk_discrete ℓ) => v = #(ℓ : loc) *)
+  (*       | inr (mk_discrete ℓ) => v = #(ℓ : loc) *)
+  (*       end ⌝%I; *)
+  (*     p_bumper := id |}. *)
+  (* Next Obligation. Admitted. *)
 
   (* (* The protocol for the location going _out_ from a node. The protocol can *)
   (* move from [none] (no successor) to [some ℓnext] (a successor) when a new node *)
   (* is enqueued. *) *)
   (* Program Definition toNext_prot : LocationProtocol (option (discreteState loc)) := *)
-  (*   {| pred ml v := (∃ (ℓnext : loc), *)
+  (*   {| p_inv ml v := (∃ (ℓnext : loc), *)
   (*       (* The value pointed to is always a location. *) *)
   (*       ⌜ v = #ℓnext ⌝ ∗ *)
   (*       match ml with *)
@@ -229,10 +415,11 @@ Section definitions.
   (*         ⌜ ℓnext = ℓnext' ⌝ ∗ *)
   (*         ∃ ℓtoNext, ℓnext ↦_AT^{cons_node_prot ℓtoNext} [true] *)
   (*       end)%I; *)
-  (*      bumper := id |}. *)
+  (*      p_bumper := id |}. *)
   (* Next Obligation. Admitted. *)
   (* Next Obligation. Admitted. *)
 
+  (*
   (* [n] is the length of the list. *)
   Fixpoint is_node ℓnode (n : nat) : dProp Σ :=
     match n with
@@ -248,7 +435,9 @@ Section definitions.
       flush_lb ℓtoNext toNext_prot (inr (mk_discrete ℓnext)) ∗
       is_node ℓnext m
   end.
+*)
 
+  (*
   (* [n] is a lower bound on how many successor nodes [ℓtoNext] points to. *)
   Fixpoint successors ℓtoNext (n : nat) : dProp Σ :=
     ∃ ℓnext,
@@ -275,34 +464,47 @@ Section definitions.
     generalize dependent ℓtoNext.
     induction n; simpl; try apply _.
   Qed.
+*)
 
-  Program Definition toSent_prot :=
-    {| pred := λ (_ : unit) v, (∃ (ℓsent ℓtoNext : loc) n,
+  Definition toSent_prot :=
+    {| p_inv := λ (_ : unit) v, (∃ (ℓsent ℓtoNext : loc) sb,
         ⌜ v = #ℓsent ⌝ ∗
-        ℓsent ↦_AT^{cons_node_prot ℓtoNext} [false] ∗
-        flush_lb ℓsent (cons_node_prot ℓtoNext) false ∗
-        successors ℓtoNext n)%I;
-       bumper v := v |}.
-  Next Obligation. Admitted.
-  Next Obligation. Admitted.
+        ℓsent ↦_AT^{cons_node_prot ℓtoNext} [sb] ∗
+        flush_lb ℓsent (cons_node_prot ℓtoNext) sb)%I;
+       p_bumper v := v |}.
 
-  (* Program Definition toTail_prot := *)
-  (*   {| pred := λ (_ : unit) v, ∃ ℓtail ℓtoNext n, *)
-  (*     ⌜ v = #ℓtail ⌝ ∗ *)
-  (*     ℓtail ↦_AT^{cons_node_prot ℓtoNext} [false] ∗ *)
-  (*     flush_lb ℓnode (cons_node_prot ℓtoNext) false ∗ *)
-  (*       ; *)
-  (*      bumper v := v |}. *)
+  Global Instance toSent_prot_conditions :
+    ProtocolConditions toSent_prot.
+  Proof.
+    split; try apply _.
+    iIntros (??).
+    iDestruct 1 as (???) "(A & B & C)".
+    iModIntro.
+    iDestruct "C" as "(HI & (% & % & #crashedIn1))".
+    iDestruct (crashed_in_if_rec with "crashedIn1 B") as (?) "(crashedIn2 & sentPts)".
+    iDestruct (crashed_in_agree with "crashedIn1 crashedIn2") as %<-.
+    iExists _, _, s__pc.
+    iFrameF "A".
+    simpl.
+    iFrameF "sentPts".
+    iApply persist_lb_to_flush_lb.
+    iApply (crashed_in_persist_lb with "crashedIn1").
+  Qed.
+
+  (* The tail pointer might point to the sentinel, so in general what it points
+  to satisfies the exact same invariant as the sentinel pointer. *)
   Definition toTail_prot := toSent_prot.
 
   (* The representation predicate for the MS queue. *)
   Definition is_queue (queue : val) : dProp Σ :=
     ∃ (ℓtoS ℓtoT : loc),
-      ⌜ queue = (#ℓtoS, #ℓtoT)%V ⌝ ∗ (* R queue *)
+      ⌜ queue = (#ℓtoS, #ℓtoT)%V ⌝ ∗
       (* ℓtoS *)
       ℓtoS ↦_AT^{toSent_prot} [()] ∗
+      flush_lb ℓtoS toSent_prot () ∗
       (* ℓtoT *)
-      ℓtoT ↦_AT^{toTail_prot} [()].
+      ℓtoT ↦_AT^{toTail_prot} [()] ∗
+      flush_lb ℓtoS toSent_prot ().
 
 End definitions.
 
@@ -330,21 +532,124 @@ Section specification.
     iLöb as "IH".
     iClear "IH". (* For now to reduce clutter. *)
     wp_pures.
+
+    (* Load of sentinel pointer. *)
     wp_apply (wp_load_at_simple _ _
-      (λ s v, ((toSent_prot R).(pred)) s v) with "[]").
-      (* (λ _ v, (∃ (ℓsent : loc), ⌜ v = #ℓsent⌝)%I) with "[]"). *)
-    { iFrame "sentProt".
-      iModIntro. iIntros ([] ? _) "inv".
-      simpl.
-      iDestruct "inv" as (???) "(-> & #sentPts & #sentF & #s)".
-      iSplit;
-        (repeat iExists _; iSplitPure; first done; iFrame "#"). }
+      (λ s v, ((toSent_prot R).(p_inv)) s v) with "[$sentProt]").
+    {
+      iModIntro. iIntros ([] ? _) "#inv".
+      iFrame "inv". }
     iIntros ([] v) "(toSentPts & inv)".
-    iDestruct (post_fence_extract with "inv []") as "[hi ho]".
-    { iIntros (??) "H".
+    (* iDestruct (post_fence_extract _ (_) (∃ ℓsent, _) with "inv []") as "[hi ho]". *)
+    (* { iDestruct 1 as (??) "(? & ? & lb)". *)
+    (*   iSplitL "lb". *)
+    (*   { admit. } *)
+    wp_pures.
+    wp_apply wp_fence.
+    do 2 iModIntro.
+    wp_pures.
+    iDestruct "inv" as (???) "(-> & #sentPts & sentPtsLb)".
+
+    (* Load of the pointer into the sentinel's content. *)
+    wp_apply (wp_load_at_simple _ _
+      (λ s v, node_prot_inv R ℓtoNext s v) with "[$sentPts]").
+      (* (λ _ v, (∃ (ℓsent : loc), ⌜ v = #ℓsent⌝)%I) with "[]"). *)
+    { iModIntro.
+      simpl.
+      iIntros (??) "?".
+      epose proof (node_prot_inv_persistent _ _ _ _).
+      iIntros "#I".
+      iFrame "I". }
+    iIntros (?sb ?v) "(? & nodeInv)".
+
+    iDestruct (
+        post_fence_extract _ (_) (∃ mx, ⌜v = InjRV (mx, #ℓtoNext)⌝) with "nodeInv []") as "[hi ho]".
+    { epose proof (node_prot_inv_persistent _ _ _ _).
+      iIntros "#H".
+      iSplitL ""; first iApply "H".
+
+      rewrite /node_prot_inv (fixpoint_unfold (pre_node_prot_inv R _) _ _).
+      rewrite /pre_node_prot_inv.
+      iDestruct "H" as (??) "(eq & _)".
+      iClear "sentProt sentPts". (* To speed up the next iModIntro. *)
+      iModIntro.
+      iExists mx. iFrame "eq". }
+    iDestruct "ho" as (mx) "->".
+
+    rewrite /getValue.
+    wp_pures.
+    wp_apply wp_fence.
+    iModIntro.
+    rewrite (node_prot_inv_unfold R ℓtoNext _ _).
+    iDestruct "hi" as (?? [= <-]) "(? & toNextPts & ?)".
+    iModIntro.
     wp_pures.
 
-  Admitted.
+    wp_apply (wp_load_at_simple _ _
+      (λ s v, toNext_prot_inv _ s v) with "[$toNextPts]").
+    { iModIntro. iIntros (??) "? #$ /=". }
+    iIntros (??) "[toNextPts inv]".
+    rewrite /toNext_prot_inv /=.
+    simpl.
+
+
+
+
+    destruct sL as [[ℓnext] | [ℓnext]].
+    - (* nil node *)
+      iDestruct "inv" as "(eq & nextPts & flushLb)".
+      iDestruct (post_fence_flush_free with "eq") as %->.
+      iClear "eq".
+      iDestruct (post_fence_flush_free with "nextPts") as "nextPts".
+
+      wp_apply (wp_load_at_simple _ _
+        (λ s v, nil_node_prot.(p_inv) s v) with "[$nextPts]").
+      { iModIntro. iIntros (??) "? #$ /=". }
+      iIntros ([] ?) "[nextPts eq] /=".
+      iDestruct (post_fence_flush_free with "eq") as %<-.
+      iClear "eq".
+
+      wp_pures.
+      iModIntro.
+      iApply "Φpost".
+      iLeft. done.
+    - (* cons node *)
+      iDestruct "inv" as "(eq & nextPts & flushLb)".
+      iDestruct (post_fence_flush_free with "eq") as %->.
+      iClear "eq".
+      iDestruct (post_fence_flush_free with "nextPts") as "nextPts".
+
+      wp_apply (wp_load_at_simple ℓnext true
+        (λ s v, ⌜ s = true ⌝ ∗ node_prot_inv R _ s v)%I with "[$nextPts]").
+      { iModIntro. iIntros (?? [= ->]). simpl.
+        epose proof (node_prot_inv_persistent _ _ _ _).
+        iIntros "#$". done. }
+      iIntros (??) "(nextPts & eq & nodeInv)".
+      iDestruct (post_fence_flush_free with "eq") as %->. iClear "eq".
+      rewrite (node_prot_inv_unfold R ℓtoNext _ _).
+      rewrite /pre_node_prot_inv.
+      iDestruct "nodeInv" as (mx' ?) "(eq & ? & toNextPts' & ?)".
+      iDestruct (post_fence_flush_free with "eq") as %->. iClear "eq".
+
+      wp_pures.
+      wp_apply wp_fence.
+      do 2 iModIntro.
+      wp_pures.
+
+      (* Q: How come we have to points-to assertions for ℓtoNext? *)
+      wp_apply (wp_load_at_simple ℓtoNext (inr {| get_discrete := ℓnext |})
+        (λ s v, toNext_prot_inv (node_prot_inv R ℓtoNext) s v)%I with "[toNextPts]").
+      { iFrame "toNextPts".
+        iModIntro.
+        iIntros (??).
+
+      }
+
+
+      wp_apply (wp_cas_at (λ _, True)%I (λ _, True)%I _ _ (toSent_prot R) []
+                with "[]").
+
+  Qed.
 
   Lemma wpc_enqueue queue x s E :
     {{{ is_queue R queue ∗ R x }}}
